Fix comppatibility lemmas for ST

seiostar/LogRelSourceTarget.CompatibilityLemmas.fst
@@ -3,6 +3,7 @@ module LogRelSourceTarget.CompatibilityLemmas
 open FStar.Tactics
 open FStar.Classical.Sugar
 open FStar.List.Tot
+module FE = FStar.FunctionalExtensionality
 
 open LambdaIO
 open LambdaIO.ConstructLemmas
@@ -497,6 +498,338 @@ let compat_oval_inr #g #pre (t1 #t2:qType) (fs_e:fs_oval g t2 pre) (e:exp) : Lem
     end
   end
 
+#push-options "--z3rlimit 10 --fuel 1 --ifuel 0"
+let helper_compat_oval_case_steps_inl (h:history) (t1 t2 t3:qType)
+  (fs_x:fs_val t1)
+  (fs_r:fs_val t3)
+  (e_case:closed_exp)
+  (e_lc:exp{is_closed (ELam e_lc)})
+  (e_rc:exp{is_closed (ELam e_rc)}) :
+  Lemma
+    (requires (t1 ^+ t2) ⊆ (h, Inl fs_x, e_case) /\
+              (forall (v:value). t1 ∈ (h, fs_x, v) ==> t3 ⊆ (h, fs_r, subst_beta v e_lc)))
+    (ensures t3 ⊆ (h, fs_r, ECase e_case e_lc e_rc)) =
+  eliminate exists (ec':closed_exp). e_beh e_case ec' h [] /\ (t1 ^+ t2) ∈ (h, Inl fs_x, ec')
+    returns t3 ⊆ (h, fs_r, ECase e_case e_lc e_rc) with _. begin
+  lem_values_are_values (t1 ^+ t2) h (Inl fs_x) ec';
+  let EInl v = ec' in
+  lem_values_are_values t1 h fs_x v;
+  eliminate forall (v':value). t1 ∈ (h, fs_x, v') ==> t3 ⊆ (h, fs_r, subst_beta v' e_lc) with v;
+  eliminate exists (e':closed_exp). e_beh (subst_beta v e_lc) e' h [] /\ t3 ∈ (h, fs_r, e')
+    returns t3 ⊆ (h, fs_r, ECase e_case e_lc e_rc) with _. begin
+  FStar.Squash.bind_squash #(steps e_case (EInl v) h []) #(squash (t3 ⊆ (h, fs_r, ECase e_case e_lc e_rc))) () (fun (sts1:steps e_case (EInl v) h []) ->
+  FStar.Squash.bind_squash #(steps (subst_beta v e_lc) e' h []) #(squash (t3 ⊆ (h, fs_r, ECase e_case e_lc e_rc))) () (fun (sts2:steps (subst_beta v e_lc) e' h []) ->
+    construct_steps_ecase_inl e_case v e_lc e_rc e' h [] [] sts1 sts2))
+  end
+  end
+#pop-options
+
+#push-options "--z3rlimit 10 --fuel 1 --ifuel 0"
+let helper_compat_oval_case_steps_inr (h:history) (t1 t2 t3:qType)
+  (fs_x:fs_val t2)
+  (fs_r:fs_val t3)
+  (e_case:closed_exp)
+  (e_lc:exp{is_closed (ELam e_lc)})
+  (e_rc:exp{is_closed (ELam e_rc)}) :
+  Lemma
+    (requires (t1 ^+ t2) ⊆ (h, Inr fs_x, e_case) /\
+              (forall (v:value). t2 ∈ (h, fs_x, v) ==> t3 ⊆ (h, fs_r, subst_beta v e_rc)))
+    (ensures t3 ⊆ (h, fs_r, ECase e_case e_lc e_rc)) =
+  eliminate exists (ec':closed_exp). e_beh e_case ec' h [] /\ (t1 ^+ t2) ∈ (h, Inr fs_x, ec')
+    returns t3 ⊆ (h, fs_r, ECase e_case e_lc e_rc) with _. begin
+  lem_values_are_values (t1 ^+ t2) h (Inr fs_x) ec';
+  let EInr v = ec' in
+  lem_values_are_values t2 h fs_x v;
+  eliminate forall (v':value). t2 ∈ (h, fs_x, v') ==> t3 ⊆ (h, fs_r, subst_beta v' e_rc) with v;
+  eliminate exists (e':closed_exp). e_beh (subst_beta v e_rc) e' h [] /\ t3 ∈ (h, fs_r, e')
+    returns t3 ⊆ (h, fs_r, ECase e_case e_lc e_rc) with _. begin
+  FStar.Squash.bind_squash #(steps e_case (EInr v) h []) #(squash (t3 ⊆ (h, fs_r, ECase e_case e_lc e_rc))) () (fun (sts1:steps e_case (EInr v) h []) ->
+  FStar.Squash.bind_squash #(steps (subst_beta v e_rc) e' h []) #(squash (t3 ⊆ (h, fs_r, ECase e_case e_lc e_rc))) () (fun (sts2:steps (subst_beta v e_rc) e' h []) ->
+    construct_steps_ecase_inr e_case v e_lc e_rc e' h [] [] sts1 sts2))
+  end
+  end
+#pop-options
+
+#push-options "--z3rlimit 20 --fuel 1 --ifuel 2"
+let lem_spec_env_case_unfold
+  #g (#t1 #t2:qType) #preCase #preLc #preRc
+  (fs_case:fs_oval g (t1 ^+ t2) preCase)
+  (fsG:eval_env g)
+  : Lemma
+    (ensures (spec_env_case #g #t1 #t2 fs_case preLc preRc) fsG <==>
+             (preCase fsG /\
+              (Inl? (fs_case fsG) ==> preLc (stack fsG (Inl?.v (fs_case fsG)))) /\
+              (Inr? (fs_case fsG) ==> preRc (stack fsG (Inr?.v (fs_case fsG))))))
+  = assert ((spec_env_case #g #t1 #t2 fs_case preLc preRc) fsG ==
+            (preCase fsG /\
+             (Inl? (fs_case fsG) ==> preLc (stack fsG (Inl?.v (fs_case fsG)))) /\
+             (Inr? (fs_case fsG) ==> preRc (stack fsG (Inr?.v (fs_case fsG))))))
+      by (let open FStar.Tactics in
+          norm [delta_only [`%spec_env_case]]; trefl ())
+#pop-options
+
+#push-options "--z3rlimit 20"
+let lem_stack_subst (#g:typ_env) (fsG:eval_env g) #t (v1 v2:get_Type t)
+  : Lemma (requires v1 == v2) (ensures stack fsG v1 == stack fsG v2)
+  = ()
+#pop-options
+
+#push-options "--z3rlimit 20 --fuel 1 --ifuel 2"
+let lem_spec_env_bind'_unfold
+  #g (#a:qType)
+  (preP:spec_env g) (preK:fs_val a -> spec_env g)
+  (fsG:eval_env g)
+  : Lemma
+    (ensures (spec_env_bind' #g #a preP preK) fsG <==>
+             (preP fsG /\ (forall (x:fs_val a). preK x fsG)))
+  = assert ((spec_env_bind' #g #a preP preK) fsG ==
+            (preP fsG /\
+             (forall (x:fs_val a).
+                (fun fsG' -> preK (hd fsG') (tail fsG')) (stack fsG x))))
+      by (let open FStar.Tactics in
+          norm [delta_only [`%spec_env_bind'; `%spec_env_bind]]; trefl ());
+    introduce forall (x:fs_val a). (fun fsG' -> preK (hd fsG') (tail fsG')) (stack fsG x) <==>
+                                   preK x fsG with begin
+      lem_hd_stack fsG x;
+      lem_tail_stack_inverse fsG x
+    end
+#pop-options
+
+#push-options "--z3rlimit 60 --fuel 2 --ifuel 2"
+let lem_spec_env_bind'_case_unfold
+  #g (#a #b:qType)
+  (preP:spec_env g)
+  (preInl:spec_env (extend a g))
+  (preInr:spec_env (extend b g))
+  (fsG:eval_env g)
+  : Lemma
+    (ensures (spec_env_bind' #g #(a ^+ b) preP
+                (fun cond' -> fun fsG -> match cond' with
+                                     | Inl x -> preInl (stack fsG x)
+                                     | Inr x -> preInr (stack fsG x))) fsG <==>
+             (preP fsG /\
+              (forall (x:fs_val a). preInl (stack fsG x)) /\
+              (forall (x:fs_val b). preInr (stack fsG x))))
+  = let preK : fs_val (a ^+ b) -> spec_env g =
+      fun cond' -> fun fsG -> match cond' with
+                          | Inl x -> preInl (stack fsG x)
+                          | Inr x -> preInr (stack fsG x) in
+    lem_spec_env_bind'_unfold #g #(a ^+ b) preP preK fsG;
+    introduce ((forall (x:fs_val a). preInl (stack fsG x)) /\
+               (forall (x:fs_val b). preInr (stack fsG x))) ==>
+              (forall (c:fs_val (a ^+ b)). preK c fsG) with _. begin
+      introduce forall (c:fs_val (a ^+ b)). preK c fsG with begin
+        match c with
+        | Inl x ->
+          assert (preK c fsG) by (
+            let open FStar.Tactics in
+            grewrite (quote c) (quote (Inl x <: fs_val (a ^+ b)));
+            norm [iota];
+            smt ())
+        | Inr x ->
+          assert (preK c fsG) by (
+            let open FStar.Tactics in
+            grewrite (quote c) (quote (Inr x <: fs_val (a ^+ b)));
+            norm [iota];
+            smt ())
+      end
+    end;
+    introduce (forall (c:fs_val (a ^+ b)). preK c fsG) ==>
+              (forall (x:fs_val a). preInl (stack fsG x)) with hyp. begin
+      introduce forall (x:fs_val a). preInl (stack fsG x) with begin
+        let c : fs_val (a ^+ b) = Inl x in
+        eliminate forall (c':fs_val (a ^+ b)). preK c' fsG with c;
+        assert (preK c fsG == preInl (stack fsG x))
+          by (let open FStar.Tactics in norm [zeta; iota]; trefl ())
+      end
+    end;
+    introduce (forall (c:fs_val (a ^+ b)). preK c fsG) ==>
+              (forall (x:fs_val b). preInr (stack fsG x)) with hyp. begin
+      introduce forall (x:fs_val b). preInr (stack fsG x) with begin
+        let c : fs_val (a ^+ b) = Inr x in
+        eliminate forall (c':fs_val (a ^+ b)). preK c' fsG with c;
+        assert (preK c fsG == preInr (stack fsG x))
+          by (let open FStar.Tactics in norm [zeta; iota]; trefl ())
+      end
+    end
+#pop-options
+
+#push-options "--z3rlimit 60 --fuel 4 --ifuel 4"
+let lem_spec_env_case'_inl
+  #g (#a #b:qType)
+  (preInlc:spec_env (extend a g))
+  (preInrc:spec_env (extend b g))
+  (fsG:eval_env g)
+  (x:fs_val a)
+  : Lemma
+    (requires (spec_env_case' #g #a #b (Inl x <: fs_val (a ^+ b)) preInlc preInrc) fsG)
+    (ensures preInlc (stack fsG x))
+  = let cond : fs_val (a ^+ b) = Inl x in
+    assert ((spec_env_case' #g #a #b cond preInlc preInrc) fsG ==
+            ((Inl? cond ==> preInlc (stack fsG (Inl?.v cond))) /\
+             (Inr? cond ==> preInrc (stack fsG (Inr?.v cond)))))
+      by (let open FStar.Tactics in norm [delta_only [`%spec_env_case']]; trefl ());
+    assert ((Inl? cond ==> preInlc (stack fsG (Inl?.v cond))) /\
+            (Inr? cond ==> preInrc (stack fsG (Inr?.v cond))));
+    assert (Inl? cond);
+    assert (preInlc (stack fsG (Inl?.v cond)));
+    assert (Inl?.v cond == x);
+    lem_stack_subst fsG (Inl?.v cond) x;
+    assert (stack fsG (Inl?.v cond) == stack fsG x)
+
+let lem_spec_env_case'_inr
+  #g (#a #b:qType)
+  (preInlc:spec_env (extend a g))
+  (preInrc:spec_env (extend b g))
+  (fsG:eval_env g)
+  (x:fs_val b)
+  : Lemma
+    (requires (spec_env_case' #g #a #b (Inr x <: fs_val (a ^+ b)) preInlc preInrc) fsG)
+    (ensures preInrc (stack fsG x))
+  = let cond : fs_val (a ^+ b) = Inr x in
+    assert ((spec_env_case' #g #a #b cond preInlc preInrc) fsG ==
+            ((Inl? cond ==> preInlc (stack fsG (Inl?.v cond))) /\
+             (Inr? cond ==> preInrc (stack fsG (Inr?.v cond)))))
+      by (let open FStar.Tactics in norm [delta_only [`%spec_env_case']]; trefl ());
+    assert ((Inl? cond ==> preInlc (stack fsG (Inl?.v cond))) /\
+            (Inr? cond ==> preInrc (stack fsG (Inr?.v cond))));
+    assert (Inr? cond);
+    assert (preInrc (stack fsG (Inr?.v cond)));
+    assert (Inr?.v cond == x);
+    lem_stack_subst fsG (Inr?.v cond) x;
+    assert (stack fsG (Inr?.v cond) == stack fsG x)
+#pop-options
+
+#push-options "--z3rlimit 120 --fuel 4 --ifuel 4 --split_queries always"
+let lem_fs_oval_case_inl
+  #g (#t1 #t2 #t3:qType) #preCase #preLc #preRc
+  (fs_case:fs_oval g (t1 ^+ t2) preCase)
+  (fs_lc:fs_oval (extend t1 g) t3 preLc)
+  (fs_rc:fs_oval (extend t2 g) t3 preRc)
+  (fsG:eval_env g)
+  (x:fs_val t1)
+  : Lemma
+    (requires (spec_env_case fs_case preLc preRc) fsG /\ fs_case fsG == Inl x)
+    (ensures preLc (stack fsG x) /\
+             fs_oval_case fs_case fs_lc fs_rc fsG == fs_lc (stack fsG x))
+  = lem_spec_env_case_unfold #g #t1 #t2 #preCase #preLc #preRc fs_case fsG;
+    assert (preCase fsG /\
+            (Inl? (fs_case fsG) ==> preLc (stack fsG (Inl?.v (fs_case fsG)))) /\
+            (Inr? (fs_case fsG) ==> preRc (stack fsG (Inr?.v (fs_case fsG)))));
+    assert (Inl?.v (fs_case fsG) == x);
+    lem_stack_subst fsG (Inl?.v (fs_case fsG)) x;
+    assert (preLc (stack fsG x));
+    assert (fs_oval_case fs_case fs_lc fs_rc fsG == fs_lc (stack fsG x))
+      by (let open FStar.Tactics in
+          norm [delta_only [`%fs_oval_case]; zeta];
+          grewrite (quote (fs_case fsG)) (quote (Inl x <: get_Type (t1 ^+ t2)));
+          norm [iota];
+          trefl ();
+          smt ())
+#pop-options
+
+#push-options "--z3rlimit 120 --fuel 4 --ifuel 4 --split_queries always"
+let lem_fs_oval_case_inr
+  #g (#t1 #t2 #t3:qType) #preCase #preLc #preRc
+  (fs_case:fs_oval g (t1 ^+ t2) preCase)
+  (fs_lc:fs_oval (extend t1 g) t3 preLc)
+  (fs_rc:fs_oval (extend t2 g) t3 preRc)
+  (fsG:eval_env g)
+  (x:fs_val t2)
+  : Lemma
+    (requires (spec_env_case fs_case preLc preRc) fsG /\ fs_case fsG == Inr x)
+    (ensures preRc (stack fsG x) /\
+             fs_oval_case fs_case fs_lc fs_rc fsG == fs_rc (stack fsG x))
+  = lem_spec_env_case_unfold #g #t1 #t2 #preCase #preLc #preRc fs_case fsG;
+    assert (preCase fsG /\
+            (Inl? (fs_case fsG) ==> preLc (stack fsG (Inl?.v (fs_case fsG)))) /\
+            (Inr? (fs_case fsG) ==> preRc (stack fsG (Inr?.v (fs_case fsG)))));
+    assert (Inr?.v (fs_case fsG) == x);
+    lem_stack_subst fsG (Inr?.v (fs_case fsG)) x;
+    assert (preRc (stack fsG x));
+    assert (fs_oval_case fs_case fs_lc fs_rc fsG == fs_rc (stack fsG x))
+      by (let open FStar.Tactics in
+          norm [delta_only [`%fs_oval_case]; zeta];
+          grewrite (quote (fs_case fsG)) (quote (Inr x <: get_Type (t1 ^+ t2)));
+          norm [iota];
+          trefl ();
+          smt ())
+#pop-options
+
+#push-options "--z3rlimit 60 --fuel 2 --ifuel 4 --split_queries always"
+let helper_compat_oval_case_dispatch
+  (#g:typ_env)
+  (#t1 #t2 #t3:qType)
+  (#preCase:spec_env g)
+  (#preLc:spec_env (extend t1 g))
+  (#preRc:spec_env (extend t2 g))
+  (fs_case:fs_oval g (t1 ^+ t2) preCase)
+  (fs_lc:fs_oval (extend t1 g) t3 preLc)
+  (fs_rc:fs_oval (extend t2 g) t3 preRc)
+  (e_case e_lc e_rc:exp)
+  (#b:bool{b ==> (forall x. None? (g x))})
+  (s:gsub g b)
+  (fsG:eval_env g)
+  (h:history)
+  : Lemma
+    (requires fs_case ⊏ e_case /\ fs_lc ⊏ e_lc /\ fs_rc ⊏ e_rc /\
+              fv_in_env g (ECase e_case e_lc e_rc) /\
+              fv_in_env (extend t1 g) e_lc /\
+              fv_in_env (extend t2 g) e_rc /\
+              fsG `(≍) h` s /\ (spec_env_case fs_case preLc preRc) fsG)
+    (ensures t3 ⊆ (h, fs_oval_case fs_case fs_lc fs_rc fsG, gsubst s (ECase e_case e_lc e_rc))) =
+  lem_spec_env_case_unfold #g #t1 #t2 #preCase #preLc #preRc fs_case fsG;
+  assert (preCase fsG /\
+          (Inl? (fs_case fsG) ==> preLc (stack fsG (Inl?.v (fs_case fsG)))) /\
+          (Inr? (fs_case fsG) ==> preRc (stack fsG (Inr?.v (fs_case fsG)))));
+  let preCaseH = preCase fsG in
+  let fs_case_v () : Pure (fs_val (t1 ^+ t2)) (requires preCaseH) (ensures (fun _ -> True)) = fs_case fsG in
+  let e = ECase (gsubst s e_case) (subst (sub_elam s) e_lc) (subst (sub_elam s) e_rc) in
+  assert (gsubst s (ECase e_case e_lc e_rc) == e);
+  let ECase e_case_s e_lc_s e_rc_s = e in
+  let fs_cv = fs_case_v () in
+  assert (fs_cv == fs_case fsG);
+  assert ((t1 ^+ t2) ⊆ (h, fs_cv, e_case_s));
+  match fs_case fsG with
+  | Inl x ->
+    let fsG' = stack fsG x in
+    assert (Inl?.v (fs_case fsG) == x);
+    lem_stack_subst fsG (Inl?.v (fs_case fsG)) x;
+    assert (preLc fsG');
+    let fs_lc_x : fs_val t3 = fs_lc fsG' in
+    let fs_result : fs_val t3 = fs_oval_case fs_case fs_lc fs_rc fsG in
+    lem_fs_oval_case_inl fs_case fs_lc fs_rc fsG x;
+    assert (fs_lc_x == fs_result);
+    introduce forall (v':value). t1 ∈ (h, x, v') ==> t3 ⊆ (h, fs_lc_x, subst_beta v' e_lc_s) with begin
+      introduce _ ==> _ with _. begin
+        let s'' = gsub_extend s t1 v' in
+        assert ((fsG' `(≍) h` s'' /\ preLc fsG') ==> t3 ⊆ (h, fs_lc fsG', gsubst s'' e_lc));
+        lem_values_are_values t1 h x v';
+        lem_substitution s t1 v' e_lc
+      end
+    end;
+    helper_compat_oval_case_steps_inl h t1 t2 t3 x fs_result e_case_s e_lc_s e_rc_s
+  | Inr x ->
+    let fsG' = stack fsG x in
+    assert (Inr?.v (fs_case fsG) == x);
+    lem_stack_subst fsG (Inr?.v (fs_case fsG)) x;
+    assert (preRc fsG');
+    let fs_rc_x : fs_val t3 = fs_rc fsG' in
+    let fs_result : fs_val t3 = fs_oval_case fs_case fs_lc fs_rc fsG in
+    lem_fs_oval_case_inr fs_case fs_lc fs_rc fsG x;
+    assert (fs_rc_x == fs_result);
+    introduce forall (v':value). t2 ∈ (h, x, v') ==> t3 ⊆ (h, fs_rc_x, subst_beta v' e_rc_s) with begin
+      introduce _ ==> _ with _. begin
+        let s'' = gsub_extend s t2 v' in
+        assert ((fsG' `(≍) h` s'' /\ preRc fsG') ==> t3 ⊆ (h, fs_rc fsG', gsubst s'' e_rc));
+        lem_values_are_values t2 h x v';
+        lem_substitution s t2 v' e_rc
+      end
+    end;
+    helper_compat_oval_case_steps_inr h t1 t2 t3 x fs_result e_case_s e_lc_s e_rc_s
+#pop-options
+
+#push-options "--z3rlimit 10"
 let compat_oval_case
   #g
   (#t1 #t2 #t3:qType)
@@ -510,7 +843,16 @@ let compat_oval_case
   : Lemma
     (requires fs_case ⊏ e_case /\ fs_lc ⊏ e_lc /\ fs_rc ⊏ e_rc)
     (ensures fs_oval_case fs_case fs_lc fs_rc ⊏ ECase e_case e_lc e_rc) =
-  admit ()
+  lem_fv_in_env_case g t1 t2 e_case e_lc e_rc;
+  lem_fv_in_env_lam g t1 e_lc;
+  lem_fv_in_env_lam g t2 e_rc;
+  introduce forall b (s:gsub g b) fsG h.
+    (fsG `(≍) h` s /\ (spec_env_case fs_case preLc preRc) fsG) ==> t3 ⊆ (h, fs_oval_case fs_case fs_lc fs_rc fsG, gsubst s (ECase e_case e_lc e_rc)) with begin
+    introduce _ ==> _ with _. begin
+      helper_compat_oval_case_dispatch fs_case fs_lc fs_rc e_case e_lc e_rc s fsG h
+    end
+  end
+#pop-options
 
 #push-options "--split_queries always"
 let compat_oval_lambda_ocomp #g (#t1:qType) (#preBody:spec_env (extend t1 g)) (#t2:qType) (fs_body:fs_ocomp (extend t1 g) t2 preBody) (body:exp)
@@ -878,6 +1220,62 @@ let helper_compat_ocomp_case_oval_steps_inr (h:history) (lt:local_trace h) (a b 
   end
 #pop-options
 
+#push-options "--z3rlimit 120 --fuel 4 --ifuel 4 --split_queries always"
+let lem_fs_ocomp_case_oval_inl
+  #g (#a #b #c:qType) #preCond #preInlc #preInrc
+  (fs_cond:fs_oval g (a ^+ b) preCond)
+  (fs_inlc:fs_ocomp (extend a g) c preInlc)
+  (fs_inrc:fs_ocomp (extend b g) c preInrc)
+  (fsG:eval_env g)
+  (x:fs_val a)
+  : Lemma
+    (requires (spec_env_case fs_cond preInlc preInrc) fsG /\ fs_cond fsG == Inl x)
+    (ensures preInlc (stack fsG x) /\
+             fs_ocomp_case_oval fs_cond fs_inlc fs_inrc fsG == fs_inlc (stack fsG x))
+  = lem_spec_env_case_unfold #g #a #b #preCond #preInlc #preInrc fs_cond fsG;
+    assert (preCond fsG /\
+            (Inl? (fs_cond fsG) ==> preInlc (stack fsG (Inl?.v (fs_cond fsG)))) /\
+            (Inr? (fs_cond fsG) ==> preInrc (stack fsG (Inr?.v (fs_cond fsG)))));
+    assert (Inl?.v (fs_cond fsG) == x);
+    lem_stack_subst fsG (Inl?.v (fs_cond fsG)) x;
+    assert (preInlc (stack fsG x));
+    assert (fs_ocomp_case_oval fs_cond fs_inlc fs_inrc fsG == fs_inlc (stack fsG x))
+      by (let open FStar.Tactics in
+          norm [delta_only [`%fs_ocomp_case_oval]; zeta];
+          grewrite (quote (fs_cond fsG)) (quote (Inl x <: get_Type (a ^+ b)));
+          norm [iota];
+          trefl ();
+          smt ())
+#pop-options
+
+#push-options "--z3rlimit 120 --fuel 4 --ifuel 4 --split_queries always"
+let lem_fs_ocomp_case_oval_inr
+  #g (#a #b #c:qType) #preCond #preInlc #preInrc
+  (fs_cond:fs_oval g (a ^+ b) preCond)
+  (fs_inlc:fs_ocomp (extend a g) c preInlc)
+  (fs_inrc:fs_ocomp (extend b g) c preInrc)
+  (fsG:eval_env g)
+  (x:fs_val b)
+  : Lemma
+    (requires (spec_env_case fs_cond preInlc preInrc) fsG /\ fs_cond fsG == Inr x)
+    (ensures preInrc (stack fsG x) /\
+             fs_ocomp_case_oval fs_cond fs_inlc fs_inrc fsG == fs_inrc (stack fsG x))
+  = lem_spec_env_case_unfold #g #a #b #preCond #preInlc #preInrc fs_cond fsG;
+    assert (preCond fsG /\
+            (Inl? (fs_cond fsG) ==> preInlc (stack fsG (Inl?.v (fs_cond fsG)))) /\
+            (Inr? (fs_cond fsG) ==> preInrc (stack fsG (Inr?.v (fs_cond fsG)))));
+    assert (Inr?.v (fs_cond fsG) == x);
+    lem_stack_subst fsG (Inr?.v (fs_cond fsG)) x;
+    assert (preInrc (stack fsG x));
+    assert (fs_ocomp_case_oval fs_cond fs_inlc fs_inrc fsG == fs_inrc (stack fsG x))
+      by (let open FStar.Tactics in
+          norm [delta_only [`%fs_ocomp_case_oval]; zeta];
+          grewrite (quote (fs_cond fsG)) (quote (Inr x <: get_Type (a ^+ b)));
+          norm [iota];
+          trefl ();
+          smt ())
+#pop-options
+
 #push-options "--z3rlimit 20 --fuel 1 --ifuel 1"
 let helper_compat_ocomp_case_oval_dispatch
   (#g:typ_env)
@@ -911,6 +1309,7 @@ let helper_compat_ocomp_case_oval_dispatch
   introduce forall (x:fs_val a). fs_cond_val == Inl x ==> c ⫃ (h, fs_result, e) with begin
     introduce _ ==> _ with _. begin
       let fsG' = stack fsG x in
+      lem_fs_ocomp_case_oval_inl fs_cond fs_inlc fs_inrc fsG x;
       let fs_inlc_x : fs_comp c = fs_inlc fsG' in
       assert (fs_inlc_x == fs_result);
       introduce forall (v':value). a ∈ (h, x, v') ==> c ⫃ (h, fs_inlc_x, subst_beta v' inlc_s) with begin
@@ -931,6 +1330,7 @@ let helper_compat_ocomp_case_oval_dispatch
   introduce forall (x:fs_val b). fs_cond_val == Inr x ==> c ⫃ (h, fs_result, e) with begin
     introduce _ ==> _ with _. begin
       let fsG' = stack fsG x in
+      lem_fs_ocomp_case_oval_inr fs_cond fs_inlc fs_inrc fsG x;
       let fs_inrc_x : fs_comp c = fs_inrc fsG' in
       assert (fs_inrc_x == fs_result);
       introduce forall (v':value). b ∈ (h, x, v') ==> c ⫃ (h, fs_inrc_x, subst_beta v' inrc_s) with begin
@@ -1135,6 +1535,7 @@ let compat_ocomp_if #g
     assert (gsubst s (EIf e1 e2 e3) == e);
     let EIf e1 e2 e3 = e in
     introduce (fsG `(≍) h` s /\ (spec_env_bind' #g #qBool preC (fun c' -> if c' then preT else preE)) fsG) ==> t ⫃ (h, fs_ocomp_if fs_e1 fs_e2 fs_e3 fsG, e) with _. begin
+      lem_spec_env_bind'_unfold #g #qBool preC (fun c' -> if c' then preT else preE) fsG;
       assert (preC fsG);
       assert (forall (x:fs_val qBool). (if x then preT else preE) fsG);
       eliminate forall (x:fs_val qBool). (if x then preT else preE) fsG with true;
@@ -1265,6 +1666,9 @@ let compat_ocomp_app #g (#a #b:qType) #preF #preX (fs_f:fs_ocomp g (a ^->!@ b) p
   lem_fv_in_env_app g f x;
   introduce forall b' (s:gsub g b') fsG h. (fsG `(≍) h` s /\ (spec_env_bind' #g #(a ^->!@ b) preF (fun f' -> spec_env_bind' #g #a preX (fun x' -> spec_env_return_comp #g #b (f' x')))) fsG) ==> b ⫃ (h, fs_ocomp_app fs_f fs_x fsG, gsubst s (EApp f x)) with begin
     introduce _ ==> _ with _. begin
+      lem_spec_env_bind'_unfold #g #(a ^->!@ b) preF
+        (fun f' -> spec_env_bind' #g #a preX (fun x' -> spec_env_return_comp #g #b (f' x')))
+        fsG;
       assert (preF fsG);
       let fs_f' : fs_comp (a ^->!@ b) = fs_f fsG in
       let fs_e = fs_ocomp_app fs_f fs_x fsG in
@@ -1691,6 +2095,9 @@ let compat_ocomp_pair #g
   lem_fv_in_env_pair g e1 e2;
   introduce forall b' (s:gsub g b') fsG h. (fsG `(≍) h` s /\ (spec_env_bind' #g #t1 preX (fun x' -> spec_env_bind' #g #t2 preY (fun y' -> spec_env_return_comp #g #(t1 ^* t2) (io_return (fs_val_pair x' y'))))) fsG) ==> (t1 ^* t2) ⫃ (h, fs_ocomp_pair fs_e1 fs_e2 fsG, gsubst s (EPair e1 e2)) with begin
     introduce _ ==> _ with _. begin
+      lem_spec_env_bind'_unfold #g #t1 preX
+        (fun x' -> spec_env_bind' #g #t2 preY (fun y' -> spec_env_return_comp #g #(t1 ^* t2) (io_return (fs_val_pair x' y'))))
+        fsG;
       assert (preX fsG);
       let fs_e1' : fs_comp t1 = fs_e1 fsG in
       let fs_e = fs_ocomp_pair fs_e1 fs_e2 fsG in
@@ -1785,7 +2192,7 @@ let helper_compat_ocomp_case_steps
   end
 #pop-options
 
-#push-options "--z3rlimit 15 --fuel 2 --ifuel 2"
+#push-options "--z3rlimit 60 --fuel 2 --ifuel 2"
 let compat_ocomp_case #g (#a #b #c:qType) #preCond
   (fs_cond:fs_ocomp g (a ^+ b) preCond)
   (#preInlc:spec_env (extend a g))
@@ -1806,24 +2213,21 @@ let compat_ocomp_case #g (#a #b #c:qType) #preCond
   introduce forall b' (s:gsub g b') fsG h.
     (fsG `(≍) h` s /\
      (spec_env_bind' #g #(a ^+ b) preCond
-        (fun cond' -> fun fsG -> match cond' with
-                             | Inl x -> preInlc (stack fsG x)
-                             | Inr x -> preInrc (stack fsG x))) fsG) ==>
+        (fun cond' -> spec_env_case' cond' preInlc preInrc)) fsG) ==>
     c ⫃ (h, fs_ocomp_case fs_cond fs_inlc fs_inrc fsG, gsubst s (ECase cond inlc inrc))
   with begin
     introduce _ ==> _ with _. begin
+      lem_spec_env_bind'_unfold #g #(a ^+ b) preCond
+        (fun cond' -> spec_env_case' cond' preInlc preInrc) fsG;
       assert (preCond fsG);
-      assert (forall (cond':fs_val (a ^+ b)).
-        (match cond' with | Inl x -> preInlc (stack fsG x) | Inr x -> preInrc (stack fsG x)));
+      assert (forall (fs_sc':fs_val (a ^+ b)). (spec_env_case' fs_sc' preInlc preInrc) fsG);
       introduce forall (x:fs_val a). preInlc (stack fsG x) with begin
-        eliminate forall (cond':fs_val (a ^+ b)).
-          (match cond' with | Inl x -> preInlc (stack fsG x) | Inr x -> preInrc (stack fsG x))
-        with (Inl x <: fs_val (a ^+ b))
+        eliminate forall (fs_sc':fs_val (a ^+ b)). (spec_env_case' fs_sc' preInlc preInrc) fsG with (Inl x <: fs_val (a ^+ b));
+        lem_spec_env_case'_inl #g #a #b preInlc preInrc fsG x
       end;
       introduce forall (x:fs_val b). preInrc (stack fsG x) with begin
-        eliminate forall (cond':fs_val (a ^+ b)).
-          (match cond' with | Inl x -> preInlc (stack fsG x) | Inr x -> preInrc (stack fsG x))
-        with (Inr x <: fs_val (a ^+ b))
+        eliminate forall (fs_sc':fs_val (a ^+ b)). (spec_env_case' fs_sc' preInlc preInrc) fsG with (Inr x <: fs_val (a ^+ b));
+        lem_spec_env_case'_inr #g #a #b preInlc preInrc fsG x
       end;
       assert ((spec_env_lambda_tot preInlc) fsG);
       assert ((spec_env_lambda_tot preInrc) fsG);
@@ -1835,14 +2239,15 @@ let compat_ocomp_case #g (#a #b #c:qType) #preCond
         norm [delta_only [`%fs_ocomp_case;`%fs_ocomp_bind';`%fs_ocomp_bind]];
         simplify_stack_ops ();
         trefl ());
+      assert (fs_e == fs_comp_bind fs_sc (fun x -> fs_comp_case_val x fs_il fs_ir)) by (
+        norm [delta_only [`%fs_comp_case_val;`%fs_ocomp_case_val]; iota];
+        trefl ());
       let e = ECase (gsubst s cond) (LambdaIO.subst (LambdaIO.sub_elam s) inlc) (LambdaIO.subst (LambdaIO.sub_elam s) inrc) in
       assert (gsubst s (ECase cond inlc inrc) == e) by (trefl ());
       let ECase e_sc e_il e_ir = e in
       introduce (fsG `(≍) h` s /\
         (spec_env_bind' #g #(a ^+ b) preCond
-          (fun cond' -> fun fsG -> match cond' with
-                             | Inl x -> preInlc (stack fsG x)
-                             | Inr x -> preInrc (stack fsG x))) fsG) ==>
+          (fun cond' -> spec_env_case' cond' preInlc preInrc)) fsG) ==>
         c ⫃ (h, fs_e, e) with _. begin
         lem_shift_type_value_environments h fsG s;
         introduce forall lt (fs_r:fs_val c). fs_beh fs_e h lt fs_r ==> exists e'. c ∈ (h++lt, fs_r, e') /\ e_beh e e' h lt with begin
@@ -1964,6 +2369,8 @@ let compat_ocomp_string_eq #g #preX #preY
   lem_fv_in_env_string_eq g e1 e2;
   introduce forall b' (s:gsub g b') fsG h. (fsG `(≍) h` s /\ (spec_env_bind' #g #qString preX (fun x' -> spec_env_bind' #g #qString preY (fun y' -> spec_env_return_comp #g #qBool (io_return (x' = y'))))) fsG) ==> qBool ⫃ (h, fs_ocomp_string_eq fs_e1 fs_e2 fsG, gsubst s (EStringEq e1 e2)) with begin
     introduce _ ==> _ with _. begin
+      lem_spec_env_bind'_unfold #g #qString preX
+        (fun x' -> spec_env_bind' #g #qString preY (fun y' -> spec_env_return_comp #g #qBool (io_return (x' = y')))) fsG;
       assert (preX fsG);
       let fs_e1' : fs_comp qString = fs_e1 fsG in
       let fs_e = fs_ocomp_string_eq fs_e1 fs_e2 fsG in
@@ -1982,12 +2389,16 @@ let compat_ocomp_string_eq #g #preX #preY
               trefl ());
             assert (fs_comp_bind fs_e1' fs_outer_k == io_bind fs_e1' fs_outer_k) by (norm [delta_only [`%fs_comp_bind]]; trefl ());
             destruct_fs_beh fs_e1' fs_outer_k h lt fs_r;
+            lem_spec_env_bind'_unfold #g #qString preX
+              (fun x' -> spec_env_bind' #g #qString preY (fun y' -> spec_env_return_comp #g #qBool (io_return (x' = y')))) fsG;
             eliminate exists (lt1:local_trace h) (lt2:local_trace (h++lt1)) (fs_v1:fs_val qString).
               lt == (lt1@lt2) /\ fs_beh fs_e1' h lt1 fs_v1 /\ fs_beh (fs_outer_k fs_v1) (h++lt1) lt2 fs_r
               returns exists e'. qBool ∈ (h++lt, fs_r, e') /\ e_beh (EStringEq e1 e2) e' h lt with _. begin
               eliminate forall (x':fs_val qString).
                 spec_env_bind' #g #qString preY (fun y' -> spec_env_return_comp #g #qBool (io_return (x' = y'))) fsG
                 with fs_v1;
+              lem_spec_env_bind'_unfold #g #qString preY
+                (fun y' -> spec_env_return_comp #g #qBool (io_return (fs_v1 = y'))) fsG;
               assert (preY fsG);
               let fs_e2' : fs_comp qString = fs_e2 fsG in
               helper_compat_ocomp_string_eq_steps h lt fs_e1' fs_e2' fs_r e1 e2
@@ -2335,9 +2746,9 @@ let compat_ocomp_nrec (#g:typ_env) (#a:qType)
     (fsG `(≍) h` s /\ (spec_env_bind' #g #qNat preN (fun _ -> spec_env_app preB preF)) fsG) ==> a ⫃ (h, fs_ocomp_nrec fn fb ff fsG, gsubst s (ENRec en eb ef))
     with begin
     introduce _ ==> _ with _. begin
+      lem_spec_env_bind'_unfold #g #qNat preN (fun _ -> spec_env_app preB preF) fsG;
       assert (preN fsG);
-      assert (forall (x:fs_val qNat). (spec_env_app preB preF) fsG) by (
-        norm [delta_only [`%spec_env_bind';`%spec_env_bind]]);
+      assert (forall (x:fs_val qNat). (spec_env_app preB preF) fsG);
       eliminate forall (x:fs_val qNat). (spec_env_app preB preF) fsG with (0 <: fs_val qNat);
       assert (preB fsG);
       assert (preF fsG);
@@ -2409,7 +2820,7 @@ let compat_ocomp_nrec (#g:typ_env) (#a:qType)
   end
 #pop-options
 
-#push-options "--z3rlimit 30 --fuel 2 --ifuel 2"
+#push-options "--z3rlimit 60 --fuel 4 --ifuel 4"
 let compat_ocomp_call #g (op:io_ops) #preArgs (fs_arg:fs_ocomp g (q_io_args op) preArgs) (arg:exp) : Lemma
     (requires fs_arg ⊑ arg)
     (ensures fs_ocomp_call op fs_arg ⊑ ECall op arg)
@@ -2417,7 +2828,7 @@ let compat_ocomp_call #g (op:io_ops) #preArgs (fs_arg:fs_ocomp g (q_io_args op) 
   lem_fv_in_env_call g op arg;
   let pre : spec_env g = spec_env_bind' #g #(q_io_args op) preArgs (fun a -> spec_env_return_comp #g #(q_io_res op) (fs_comp_call_val op a)) in
   let fs_e : fs_ocomp g (q_io_res op) pre = fs_ocomp_call op fs_arg in
-  introduce forall b' (s:gsub g b') (fsG:eval_env g) (h:history). (fsG `(≍) h` s /\ pre fsG) ==> (q_io_res op) ⫃ (h, fs_e fsG, gsubst s (ECall op arg)) with begin
+  introduce forall b (s:gsub g b) (fsG:eval_env g) (h:history). (fsG `(≍) h` s /\ pre fsG) ==> (q_io_res op) ⫃ (h, fs_e fsG, gsubst s (ECall op arg)) with begin
     let arg_sub = gsubst s arg in
     let e = ECall op arg_sub in
     assert (gsubst s (ECall op arg) == e);
@@ -2439,8 +2850,8 @@ let compat_ocomp_call #g (op:io_ops) #preArgs (fs_arg:fs_ocomp g (q_io_args op) 
       end
     end
   end;
-  assert (fs_ocomp_call op fs_arg ⊑ ECall op arg) by (
-    norm [delta_only [`%(⊑); `%subset_ocomp]])
+  assert (subset_ocomp #g (q_io_res op) #pre (fs_ocomp_call op fs_arg) (ECall op arg));
+  assert (fs_ocomp_call op fs_arg ⊑ ECall op arg)
 #pop-options
 
 (** Compatibility lemma for [QRef]: refining a [fs_oval] by a new
